WIP trace proofs

aneris/examples/transactional_consistency/state_based_model.v
@@ -1,13 +1,14 @@
-From iris.algebra Require Import gmap gset list.
+From iris.algebra Require Import gmap list.
 From aneris.examples.transactional_consistency Require Import user_params.
 From stdpp Require Import strings.
 From aneris.aneris_lang Require Import network resources.
 
-(* The string argument below is an identifier *)
+Definition Tag : Type := string.
+
 Inductive operation : Type :=
-  | Rd (s : string) (k : Key) (ov : option val) : operation 
-  | Wr (s : string) (k : Key) (v : val) : operation
-  | Cm (s : string) (b : bool) : operation.
+  | Rd (tag : Tag) (k : Key) (ov : option val) : operation 
+  | Wr (tag : Tag) (k : Key) (v : val) : operation
+  | Cm (tag : Tag) (b : bool) : operation.
 
 #[global] Instance operation_eq_dec : EqDecision operation.
 Proof. solve_decision. Defined.
@@ -32,90 +33,147 @@ Qed.
 
 Definition transaction : Type := list operation.
 
-Definition execution : Type := list ((gmap Key val) * transaction).
+Definition tagOfOp (op : operation) : Tag :=
+  match op with 
+    | Rd tag _ _ => tag
+    | Wr tag _ _ => tag
+    | Cm tag _ => tag
+  end.
 
-Definition valid_execution (exec : execution): Prop := true.
+Definition rel_list {A : Type} (l : list A) (a1 a2 : A) : Prop :=
+  ∃ i j, i <= j ∧ l !! i = Some a1 ∧ l !! j = Some a2.
 
-Definition commitTest : Type := execution -> transaction -> bool.
+Definition valid_transaction (t : transaction) : Prop :=
+  (* The last operation is the commit operation *)
+  (∃ s b, last t = Some (Cm s b)) ∧ 
+  (* The commit operaion is unique *)
+  (∀ op s b, op ∈ t → op = Cm s b → last t = Some op) ∧
+  (* All operations use the same Tag *)
+  (∀ op1 op2, op1 ∈ t → op2 ∈ t → tagOfOp op1 = tagOfOp op2).
 
-Definition executionTest : Type := execution -> list transaction -> bool.
+Definition state : Type := gmap Key val.
 
-Definition executionTestGen (test : commitTest) : executionTest := 
-  λ (exec : execution) (transactions : list transaction), forallb (test exec) transactions.
+Definition applyTransaction (s : state) (t : transaction) : state := 
+  foldl (λ s op, match op with | Wr _ k v => <[k := v]> s | _ => s end) s t.
+  
+Definition execution : Type := list (transaction * state).
+
+Definition commitTest : Type := execution -> transaction -> Prop.
+
+Definition valid_transactions (T : list transaction) : Prop := 
+  (* Transactions read their own writes *)
+  (∀ t tag k ov, t ∈ T → 
+                  Rd tag k ov ∈ t → 
+                  ∃ v, Wr tag k v ∈ t →
+                  rel_list t (Wr tag k v) (Rd tag k ov) →
+                  (¬∃ v', Wr tag k v' ∈ t ∧ 
+                          v' ≠ v ∧ 
+                          rel_list t (Wr tag k v) (Wr tag k v') ∧
+                          rel_list t (Wr tag k v') (Rd tag k ov)) →
+                  ov = Some v) ∧ 
+  (* Transactions read from some write *)
+  (∀ t tag k v, t ∈ T → 
+                 Rd tag k (Some v) ∈ t →
+                 ∃ t' tag', t' ∈ T ∧ Wr tag' k v ∈ t') ∧
+  (* Transactions satisfy the baseline transaction contraints *)
+  (∀ t, t ∈ T → valid_transaction t).
+
+Definition valid_execution (test : commitTest) (exec : execution) : Prop :=
+  (* Transitions are valid *)
+  (∀ i e1 e2, exec !! i = Some e1 → 
+              exec !! (i + 1) = Some e2 →
+              applyTransaction e1.2 e2.1 = e2.2) ∧
+  (* Initial state is valid *)
+  (exec !! 0 = Some ([], ∅)) ∧
+  (* The commit test is satisfied *)
+  (∀ t, t ∈ (split exec).1 → test exec t).
 
 (** Read Uncommitted  *)
 
-Definition commitTestRU : commitTest := 
-  λ exec trans, true.
-
-Definition executionTestRU : executionTest := 
-  λ exec transactions, executionTestGen commitTestRU exec transactions.
+Definition commit_test_ru : commitTest := λ exec trans, true.
 
 (** Read Committed  *)
 
-Fixpoint cut_inner {A : Type} (l acc : list A) (test : A → bool) : list A := 
-  match l with 
-  | h :: t => if test h then (app acc [h]) else cut_inner t (app acc [h]) test
-  | [] => acc
-  end.
+Definition initTag : Tag := "init_tag".
 
-Definition cut {A : Type} (l : list A) (test : A → bool) : list A := cut_inner l [] test.
+Definition idOfTrans (t : transaction) : Tag :=
+  match head t with | Some op => tagOfOp op | None => initTag end.
 
-Definition transIdEquiv (s : string) (trans : transaction) : bool := 
-  match head trans with 
-  | Some op => 
-    match op with 
-    | Rd s' _ _ => bool_decide (s = s')
-    | Wr s' _ _ => bool_decide (s = s')
-    | Cm s' _ => bool_decide (s = s')
-    end
-  | None => false
-  end. 
+Definition read_state (tag : Tag) (k : Key) (ov : option val) 
+(exec : execution) (s : state) : Prop := 
+  (s ∈ (split exec).2) ∧ 
+  (s !! k = ov) ∧
+  (∀ i j s' t', (split exec).2 !! i = Some s → 
+                exec !! j = Some (t', s') →
+                tag = idOfTrans t' →
+                i <= j).
 
-Definition readStates (s : string) (k : Key) (ov : option val) 
-(exec : execution) : list ((gmap Key val) * transaction) := 
-  let priorStates := cut exec (λ e, let (_, trans) := e in transIdEquiv s trans) in 
-  filter (λ (e : (gmap Key val) * transaction), let (map, _) := e in map !! k = ov) priorStates. 
+Definition pre_read (exec : execution) (t : transaction) : Prop :=
+  ∀ op tag k ov, op ∈ t → 
+                  op = Rd tag k ov →
+                  ∃ s, read_state tag k ov exec s.
 
-Definition preRead (trans : transaction) (exec : execution): bool :=
-  forallb 
-    (λ (op : operation), match op with 
-                          | Rd s k ov => bool_decide (readStates s k ov exec ≠ []) 
-                          | _ => true 
-                         end) 
-    trans.
+Definition commit_test_rc : commitTest := 
+  λ exec trans, pre_read exec trans.
 
-Definition commitTestRC : commitTest := 
-  λ exec trans, preRead trans exec.
-
-Definition executionTestRC : executionTest := 
-  λ exec transactions, executionTestGen commitTestRC exec transactions.
-  
 (** Snapshot Isolation *)
 
-(* Definition complete (state : (gmap Key val) * transaction) (trans : transaction) 
-(exec : execution) : bool := 
-  forallb 
-    (λ (op : operation), match op with 
-                          | Rd s k ov => bool_decide (In state (readStates s k ov exec)) 
-                          | _ => true 
-                        end) 
-    trans. 
+Definition complete (exec : execution) (t : transaction)  
+(s : state): Prop := 
+  ∀ op tag k ov, op ∈ t → 
+                  op = Rd tag k ov →
+                  read_state tag k ov exec s.
 
-Definition commitTestSI : commitTest := 
-  λ exec trans, 
-    existsb (λ e, let (map, _) := e in 
-                    complete e trans exec  && 
-                    true) 
-            exec.
+Definition parent_state (exec : execution) (t : transaction) (s : state) : Prop :=
+  ∃ i t' s', exec !! i = Some (t' , s) ∧ exec !! (i + 1) = Some (t, s').
 
-Definition executionTestSI : executionTest := 
-  λ exec transactions, executionTestGen commitTestSI exec transactions. *)
+Definition no_conf (exec : execution) (t : transaction) (s : state) : Prop := 
+  ¬(∃ k, (∃ tag v, Wr tag k v ∈ t) ∧ 
+         (∀ sp, parent_state exec t sp → s !! k ≠ sp !! k)). 
 
-(** Embedding of into the trace infrastructure  *)
+Definition commit_test_si : commitTest := 
+  λ exec trans, ∃ s, s ∈ (split exec).2 ∧ 
+                complete exec trans s ∧ 
+                no_conf exec trans s.
 
-Definition valid_ru (t : list val): Prop := true.
+(** Embedding into the trace infrastructure *)
 
-Definition valid_rc (t : list val): Prop := true.
+Definition toOp (event : val) : option operation := 
+  match event with 
+    | (#(LitString tag), (#"Rd", (#(LitString k), NONEV)))%V => Some (Rd tag k None)
+    | (#(LitString tag), (#"Rd", (#(LitString k), SOMEV v)))%V => Some (Rd tag k (Some v))
+    | (#(LitString tag), (#"Wr", (#(LitString k), v)))%V => Some (Wr tag k v)
+    | (#(LitString tag), (#"Cm", #(LitBool b)))%V => Some (Cm tag b)
+    | _ => None
+  end.
 
-Definition valid_si (t : list val): Prop := true.
+Definition toEvent (op : operation) : val := 
+  match op with 
+    | Rd tag k None => (#tag, (#"Rd", (#k, NONEV)))
+    | Rd tag k (Some v) => (#tag, (#"Rd", (#k, SOMEV v)))
+    | Wr tag k v => (#tag, (#"Wr", (#k, v)))
+    | Cm tag b => (#tag, (#"Cm", #b))
+  end.
+
+Definition extractionOf (trace : list val) (T : list transaction): Prop := 
+  (* Trace and transactions contain the same operations *)
+  (∀ event op, event ∈ trace → toOp event = Some op → ∃ t, t ∈ T → op ∈ t) ∧
+  (∀ t op, t ∈ T → op ∈ t → (toEvent op) ∈ trace) ∧
+  (* Operations are grouped into transactions correctly *)
+  (∀ t op1 op2, t ∈ T → op1 ∈ t → op2 ∈ t → tagOfOp op1 = tagOfOp op2).
+
+Definition comTrans (T : list transaction) : list transaction := 
+  List.filter (λ t, match last t with | Some (Cm tag true) => true | _ => false end) T.
+
+Definition based_on (exec : execution) (transactions : list transaction) : Prop :=
+  ∀ t, t ∈ (split exec).1 ↔ t ∈ transactions.
+
+Definition valid_trace (test : commitTest) : list val → Prop :=
+  λ t, ∀ T, extractionOf t T ∧ valid_transactions T ∧ 
+            ∃ exec, based_on exec (comTrans T) ∧ valid_execution test exec.
+
+Definition valid_trace_ru : list val → Prop := valid_trace commit_test_ru.
+
+Definition valid_trace_rc : list val → Prop := valid_trace commit_test_rc.
+
+Definition valid_trace_si : list val → Prop := valid_trace commit_test_si.
